fstar/treesync/code/MLS.TreeSync.Invariants.ParentHash.fst
@@ -32,78 +32,122 @@ let get_parent_hash_of #bytes #bl #tkt #l #i t =
   | TLeaf (Some content) -> content.data.parent_hash
   | TNode (Some content) _ _ -> content.parent_hash
 
-val mem_ul: x:nat -> l:list (nat_lbytes 4) -> bool
-let rec mem_ul x l =
-  match l with
-  | [] -> false
-  | h::t -> x=h || mem_ul x t
+val max: int -> int -> int
+let max x y =
+  if x < y then y else x
 
-val un_add_unmerged_leaf: list (nat_lbytes 4) -> nat -> bool
-let un_add_unmerged_leaf leaves i =
-  not (mem_ul i leaves)
+val last_commit_epoch:
+  #bytes:Type0 -> {|bytes_like bytes|} -> #tkt:treekem_types bytes ->
+  #l:nat -> #i:tree_index l ->
+  t:treesync bytes tkt l i -> nat_lbytes 8
+let rec last_commit_epoch #bytes #bl #tkt #l #i t =
+  match t with
+  | TLeaf None -> 0
+  | TLeaf (Some ln) -> (
+    match ln.data.source with
+    | LNS_commit -> ln.data.commit_epoch
+    | _ -> 0
+  )
+  | TNode _ left right ->
+    max (last_commit_epoch left) (last_commit_epoch right)
 
-val un_add: #bytes:Type0 -> {|bytes_like bytes|} -> #tkt:treekem_types bytes -> #l:nat -> #i:tree_index l -> treesync bytes tkt l i -> list (nat_lbytes 4) -> treesync bytes tkt l i
-let un_add #bytes #bl #tkt #l #i t leaves =
-  un_addP t (un_add_unmerged_leaf leaves)
-
-val parent_hash_correct: #bytes:Type0 -> {|crypto_bytes bytes|} -> #tkt:treekem_types bytes -> #ld:nat -> #lp:nat{ld < lp} -> #id:tree_index ld -> #ip:tree_index lp{leaf_index_inside lp ip id} -> d:treesync bytes tkt ld id{node_has_parent_hash d} -> p:treesync bytes tkt lp ip{node_not_blank p} -> bool
+val parent_hash_correct:
+  #bytes:Type0 -> {|crypto_bytes bytes|} -> #tkt:treekem_types bytes ->
+  #ld:nat -> #lp:nat{ld < lp} -> #id:tree_index ld -> #ip:tree_index lp{leaf_index_inside lp ip id} ->
+  d:treesync bytes tkt ld id{node_has_parent_hash d} -> p:treesync bytes tkt lp ip{node_not_blank p} ->
+  bool
 let parent_hash_correct #bytes #cb #tkt #ld #lp #id #ip d p =
   let p_content = (Some?.v (TNode?.data p)) in
   let expected_parent_hash = get_parent_hash_of d in
   let (_, sibling) = get_child_sibling p id in
-  let original_sibling = un_add sibling p_content.unmerged_leaves in
+  let original_sibling = un_add sibling (last_commit_epoch p) in
   compute_parent_hash_pre p_content.content (length #bytes p_content.parent_hash) original_sibling &&
   expected_parent_hash = compute_parent_hash p_content.content p_content.parent_hash original_sibling
 
-val set_equal_mem: #a:eqtype -> list a -> a -> bool
-let set_equal_mem #a l x =
+val last_update_correct:
+  #bytes:Type0 -> {|bytes_like bytes|} -> #tkt:treekem_types bytes ->
+  #ld:nat -> #lp:nat{ld < lp} -> #id:tree_index ld -> #ip:tree_index lp{leaf_index_inside lp ip id} ->
+  d:treesync bytes tkt ld id -> p:treesync bytes tkt lp ip ->
+  bool
+let last_update_correct #bytes #bl #tkt #ld #lp #id #ip d p =
+  last_commit_epoch d = last_commit_epoch p
+
+val mem_flipped: #a:eqtype -> list a -> a -> bool
+let mem_flipped #a l x =
   List.Tot.mem x l
 
-val set_eq: #a:eqtype -> list a -> list a -> bool
-let set_eq #a l1 l2 =
-  List.Tot.for_all (set_equal_mem l1) l2 && List.Tot.for_all (set_equal_mem l2) l1
+val set_subset: #a:eqtype -> list a -> list a -> bool
+let set_subset #a l1 l2 =
+  List.Tot.for_all (mem_flipped l2) l1
+
+val unmerged_leaves_aux:
+  #bytes:Type0 -> {|bytes_like bytes|} -> #tkt:treekem_types bytes ->
+  #l:nat -> #i:tree_index l ->
+  epoch:nat -> t:treesync bytes tkt l i ->
+  list nat
+let rec unmerged_leaves_aux #bytes #bl #tkt #l #i epoch t =
+  match t with
+  | TLeaf None -> []
+  | TLeaf oln ->
+    if is_unmerged_leaf epoch oln then
+      [i]
+    else
+      []
+  | TNode _ left right ->
+    unmerged_leaves_aux epoch left @ unmerged_leaves_aux epoch right
+
+val unmerged_leaves:
+  #bytes:Type0 -> {|bytes_like bytes|} -> #tkt:treekem_types bytes ->
+  #l:nat -> #i:tree_index l ->
+  t:treesync bytes tkt l i ->
+  list nat
+let unmerged_leaves #bytes #bl #tkt #l #i t =
+  unmerged_leaves_aux (last_commit_epoch t) t
 
 type node_index = dtuple2 nat tree_index
 
 val nat_to_node_index: nat -> node_index
 let nat_to_node_index n = (|0, n|)
 
-val unmerged_resolution: list (nat_lbytes 4) -> list node_index
+val unmerged_resolution: list nat -> list node_index
 let unmerged_resolution l =
   List.Tot.map nat_to_node_index l
 
-val resolution: #bytes:Type0 -> {|bytes_like bytes|} -> #tkt:treekem_types bytes -> #l:nat -> #i:tree_index l -> treesync bytes tkt l i -> list node_index
+val resolution:
+  #bytes:Type0 -> {|bytes_like bytes|} -> #tkt:treekem_types bytes ->
+  #l:nat -> #i:tree_index l ->
+  treesync bytes tkt l i ->
+  list node_index
 let rec resolution #bytes #bl #tkt #l #i t =
   match t with
   | TLeaf None -> []
   | TLeaf (Some _) -> assert(l == 0); [(|l, i|)]
   | TNode None left right ->
     resolution left @ resolution right
-  | TNode (Some content) _ _ -> (|l, i|)::(unmerged_resolution content.unmerged_leaves)
+  | TNode (Some content) _ _ ->
+    (|l, i|)::(unmerged_resolution (unmerged_leaves t))
 
-val last_update_lhs: #bytes:Type0 -> {|bytes_like bytes|} -> #tkt:treekem_types bytes -> #ld:nat -> #lp:nat{ld < lp} -> #id:tree_index ld -> #ip:tree_index lp{leaf_index_inside lp ip id} -> d:treesync bytes tkt ld id -> p:treesync bytes tkt lp ip{node_not_blank p} -> list node_index
-let last_update_lhs #bytes #bl #tkt #ld #lp #id #ip d p =
+val filter_lhs: #bytes:Type0 -> {|bytes_like bytes|} -> #tkt:treekem_types bytes -> #ld:nat -> #lp:nat{ld < lp} -> #id:tree_index ld -> #ip:tree_index lp{leaf_index_inside lp ip id} -> d:treesync bytes tkt ld id -> p:treesync bytes tkt lp ip{node_not_blank p} -> list node_index
+let filter_lhs #bytes #bl #tkt #ld #lp #id #ip d p =
   let (c, _) = get_child_sibling p id in
-  List.Tot.filter (op_disEquality (|ld, id|)) (resolution c)
+  (resolution c)
 
-val last_update_rhs: #bytes:Type0 -> {|bytes_like bytes|} -> #tkt:treekem_types bytes -> #ld:nat -> #lp:nat{ld < lp} -> #id:tree_index ld -> #ip:tree_index lp{leaf_index_inside lp ip id} -> d:treesync bytes tkt ld id -> p:treesync bytes tkt lp ip{node_not_blank p} -> list node_index
-let last_update_rhs #bytes #bl #tkt #ld #lp #id #ip d p =
-  let (c, _) = get_child_sibling p id in
-  let p_unmerged_leaves = (Some?.v (TNode?.data p)).unmerged_leaves in
-  unmerged_resolution (List.Tot.filter (leaf_index_inside_tree c) p_unmerged_leaves)
+val filter_rhs: #bytes:Type0 -> {|bytes_like bytes|} -> #tkt:treekem_types bytes -> #ld:nat -> #lp:nat{ld < lp} -> #id:tree_index ld -> #ip:tree_index lp{leaf_index_inside lp ip id} -> d:treesync bytes tkt ld id -> p:treesync bytes tkt lp ip{node_not_blank p} -> list node_index
+let filter_rhs #bytes #bl #tkt #ld #lp #id #ip d p =
+  (|ld, id|)::(unmerged_resolution (unmerged_leaves p))
 
-val last_update_d_in_res_c: #bytes:Type0 -> {|bytes_like bytes|} -> #tkt:treekem_types bytes -> #ld:nat -> #lp:nat{ld < lp} -> #id:tree_index ld -> #ip:tree_index lp{leaf_index_inside lp ip id} -> d:treesync bytes tkt ld id -> p:treesync bytes tkt lp ip{node_not_blank p} -> bool
-let last_update_d_in_res_c #bytes #bl #tkt #ld #lp #id #ip d p =
+val filter_d_in_res_c: #bytes:Type0 -> {|bytes_like bytes|} -> #tkt:treekem_types bytes -> #ld:nat -> #lp:nat{ld < lp} -> #id:tree_index ld -> #ip:tree_index lp{leaf_index_inside lp ip id} -> d:treesync bytes tkt ld id -> p:treesync bytes tkt lp ip{node_not_blank p} -> bool
+let filter_d_in_res_c #bytes #bl #tkt #ld #lp #id #ip d p =
   let (c, _) = get_child_sibling p id in
   List.Tot.mem (|ld, id|) (resolution c)
 
-val last_update_correct: #bytes:Type0 -> {|bytes_like bytes|} -> #tkt:treekem_types bytes -> #ld:nat -> #lp:nat{ld < lp} -> #id:tree_index ld -> #ip:tree_index lp{leaf_index_inside lp ip id} -> d:treesync bytes tkt ld id -> p:treesync bytes tkt lp ip{node_not_blank p} -> bool
-let last_update_correct #bytes #bl #tkt #ld #lp #id #ip d p =
-  last_update_d_in_res_c d p && set_eq (last_update_lhs d p) (last_update_rhs d p)
+val filter_correct: #bytes:Type0 -> {|bytes_like bytes|} -> #tkt:treekem_types bytes -> #ld:nat -> #lp:nat{ld < lp} -> #id:tree_index ld -> #ip:tree_index lp{leaf_index_inside lp ip id} -> d:treesync bytes tkt ld id -> p:treesync bytes tkt lp ip{node_not_blank p} -> bool
+let filter_correct #bytes #bl #tkt #ld #lp #id #ip d p =
+  filter_d_in_res_c d p && set_subset (filter_lhs d p) (filter_rhs d p)
 
 val parent_hash_linked: #bytes:Type0 -> {|crypto_bytes bytes|} -> #tkt:treekem_types bytes -> #ld:nat -> #lp:nat{ld < lp} -> #id:tree_index ld -> #ip:tree_index lp{leaf_index_inside lp ip id} -> d:treesync bytes tkt ld id{node_has_parent_hash d} -> p:treesync bytes tkt lp ip{node_not_blank p} -> bool
 let parent_hash_linked #bytes #cb #tkt #ld #lp #id #ip d p =
-  parent_hash_correct d p && last_update_correct d p
+  parent_hash_correct d p && last_update_correct d p && filter_correct d p
 
 val node_has_parent_hash_link_aux: #bytes:Type0 -> {|crypto_bytes bytes|} -> #tkt:treekem_types bytes -> #ld:nat -> #lp:nat{ld < lp} -> #id:tree_index ld -> #ip:tree_index lp{leaf_index_inside lp ip id} -> d:treesync bytes tkt ld id -> p:treesync bytes tkt lp ip{node_not_blank p} -> bool
 let rec node_has_parent_hash_link_aux #bytes #cb #tkt #ld #lp #id #ip d p =
