fstar/treesync/code/MLS.TreeSync.Invariants.Epoch.fst
@@ -1,0 +1,30 @@
+module MLS.TreeSync.Invariants.Epoch
+
+open Comparse
+open MLS.Tree
+open MLS.TreeSync.NetworkTypes
+open MLS.TreeSync.Types
+
+val leaf_node_epoch:
+  #bytes:Type0 -> {|bytes_like bytes|} -> #tkt:treekem_types bytes ->
+  leaf_node_nt bytes tkt ->
+  nat_lbytes 8
+let leaf_node_epoch #bytes #bl #tkt ln =
+  match ln.data.source with
+  | LNS_key_package -> ln.add_epoch
+  | LNS_update -> ln.data.update_epoch
+  | LNS_commit -> ln.data.commit_epoch
+
+val epoch_invariant:
+  #bytes:Type0 -> {|bytes_like bytes|} -> #tkt:treekem_types bytes ->
+  #l:nat -> #i:tree_index l ->
+  nat -> treesync bytes tkt l i ->
+  bool
+let rec epoch_invariant #bytes #bl #tkt #l #i epoch t =
+  match t with
+  | TLeaf None ->
+    true
+  | TLeaf (Some ln) ->
+    leaf_node_epoch ln <= epoch
+  | TNode _ left right ->
+    epoch_invariant epoch left && epoch_invariant epoch right
