fstar/treesync/proofs/MLS.TreeSync.Invariants.Epoch.Proofs.fst
@@ -1,0 +1,182 @@
+module MLS.TreeSync.Invariants.Epoch.Proofs
+
+open Comparse
+open MLS.Crypto
+open MLS.NetworkTypes
+open MLS.Tree
+open MLS.TreeSync.NetworkTypes
+open MLS.TreeSync.Types
+open MLS.TreeSync.Operations
+open MLS.TreeSync.Invariants.Epoch
+open MLS.TreeSync.ParentHash
+open MLS.TreeCommon
+//open MLS.TreeCommon.Lemmas
+//open MLS.MiscLemmas
+
+#set-options "--fuel 1 --ifuel 1"
+
+(*** Create ***)
+
+val epoch_invariant_tree_create:
+  #bytes:Type0 -> {|bytes_like bytes|} -> #tkt:treekem_types bytes ->
+  epoch:nat -> ln:leaf_node_nt bytes tkt ->
+  Lemma
+  (requires leaf_node_epoch ln == 0)
+  (ensures epoch_invariant epoch (tree_create (Some ln)))
+let epoch_invariant_tree_create #bytes #bl #tkt epoch ln = ()
+
+(*** Update/Remove ***)
+
+val epoch_invariant_tree_change_path:
+  #bytes:Type0 -> {|bytes_like bytes|} -> #tkt:treekem_types bytes ->
+  #l:nat -> #i:tree_index l ->
+  epoch:nat ->
+  t:treesync bytes tkt l i -> li:leaf_index l i -> oln:option (leaf_node_nt bytes tkt) -> Lemma
+  (requires
+    epoch_invariant epoch t /\
+    (Some? oln ==> leaf_node_epoch (Some?.v oln) <= epoch)
+  )
+  (ensures epoch_invariant epoch (tree_change_path t li oln None))
+let rec epoch_invariant_tree_change_path #l #i epoch t li oln =
+  match t with
+  | TLeaf _ -> ()
+  | TNode _ left right ->
+    if is_left_leaf li then
+      epoch_invariant_tree_change_path epoch left li oln
+    else
+      epoch_invariant_tree_change_path epoch right li oln
+
+val epoch_invariant_tree_update:
+  #bytes:Type0 -> {|bytes_like bytes|} -> #tkt:treekem_types bytes ->
+  #l:nat -> #i:tree_index l ->
+  epoch:nat ->
+  t:treesync bytes tkt l i -> li:leaf_index l i -> ln:leaf_node_nt bytes tkt ->
+  Lemma
+  (requires
+    epoch_invariant epoch t /\
+    leaf_node_epoch ln <= epoch
+  )
+  (ensures epoch_invariant epoch (tree_update t li ln))
+let epoch_invariant_tree_update #l #i epoch t li ln =
+  epoch_invariant_tree_change_path epoch t li (Some ln)
+
+val epoch_invariant_tree_remove:
+  #bytes:Type0 -> {|bytes_like bytes|} -> #tkt:treekem_types bytes ->
+  #l:nat -> #i:tree_index l ->
+  epoch:nat ->
+  t:treesync bytes tkt l i -> li:leaf_index l i ->
+  Lemma
+  (requires epoch_invariant epoch t)
+  (ensures epoch_invariant epoch (tree_remove t li))
+let epoch_invariant_tree_remove #l #i epoch t li =
+  epoch_invariant_tree_change_path epoch t li None
+
+(*** Extend / Truncate ***)
+
+val epoch_invariant_mk_blank_tree:
+  #bytes:Type0 -> {|bl:bytes_like bytes|} -> #tkt:treekem_types bytes ->
+  epoch:nat ->
+  l:nat -> i:tree_index l ->
+  Lemma (ensures epoch_invariant #bytes #bl #tkt epoch (mk_blank_tree l i))
+let rec epoch_invariant_mk_blank_tree #bytes #bl #tkt epoch l i =
+  if l = 0 then ()
+  else (
+    epoch_invariant_mk_blank_tree #bytes #bl #tkt epoch (l-1) (left_index i);
+    epoch_invariant_mk_blank_tree #bytes #bl #tkt epoch (l-1) (right_index i)
+  )
+
+val epoch_invariant_tree_extend:
+  #bytes:Type0 -> {|bytes_like bytes|} -> #tkt:treekem_types bytes ->
+  #l:nat ->
+  epoch:nat ->
+  t:treesync bytes tkt l 0 ->
+  Lemma
+  (requires epoch_invariant epoch t)
+  (ensures epoch_invariant epoch (tree_extend t))
+let epoch_invariant_tree_extend #bytes #bl #tkt #l epoch t =
+  epoch_invariant_mk_blank_tree #bytes #bl #tkt epoch l (right_index #(l+1) 0)
+
+val epoch_invariant_tree_truncate:
+  #bytes:Type0 -> {|bytes_like bytes|} -> #tkt:treekem_types bytes ->
+  #l:pos ->
+  epoch:nat ->
+  t:treesync bytes tkt l 0{is_tree_empty (TNode?.right t)} -> Lemma
+  (requires epoch_invariant epoch t)
+  (ensures epoch_invariant epoch (tree_truncate t))
+let epoch_invariant_tree_truncate #bytes #bl #tkt #l epoch t =
+  ()
+
+(*** Add ***)
+
+val epoch_invariant_tree_add:
+  #bytes:Type0 -> {|bytes_like bytes|} -> #tkt:treekem_types bytes ->
+  #l:nat -> #i:tree_index l ->
+  epoch:nat_lbytes 8 ->
+  t:treesync bytes tkt l i -> li:leaf_index l i -> content:leaf_node_nt bytes tkt{content.data.source == LNS_key_package} ->
+  Lemma
+  (requires epoch_invariant epoch t)
+  (ensures epoch_invariant epoch (tree_add epoch t li content))
+let rec epoch_invariant_tree_add #bytes #bl #tkt #l #i epoch t li content =
+  match t with
+  | TLeaf _ -> ()
+  | TNode opt_content left right -> (
+    if is_left_leaf li then
+      epoch_invariant_tree_add epoch left li content
+    else
+      epoch_invariant_tree_add epoch right li content
+  )
+
+(*** Apply path ***)
+
+val epoch_invariant_apply_path_aux:
+  #bytes:Type0 -> {|crypto_bytes bytes|} -> #tkt:treekem_types bytes ->
+  #l:nat -> #i:tree_index l -> #li:leaf_index l i ->
+  epoch:nat ->
+  t:treesync bytes tkt l i -> p:pathsync bytes tkt l i li -> parent_parent_hash:mls_bytes bytes ->
+  Lemma
+  (requires
+    apply_path_aux_pre #bytes t p (length #bytes parent_parent_hash) /\
+    leaf_node_epoch (get_path_leaf p) <= epoch /\
+    epoch_invariant epoch t
+  )
+  (ensures epoch_invariant epoch (apply_path_aux t p parent_parent_hash))
+let rec epoch_invariant_apply_path_aux #bytes #cb #tkt #l #i #li epoch t p parent_parent_hash =
+  match t, p with
+  | TLeaf _, PLeaf ext_content -> ()
+  | TNode _ left right, PNode opt_ext_content p_next ->
+    let (child, sibling) = get_child_sibling t li in
+    let (new_opt_content, new_parent_parent_hash) = compute_new_np_and_ph opt_ext_content sibling parent_parent_hash in
+    if is_left_leaf li then
+      epoch_invariant_apply_path_aux epoch left p_next new_parent_parent_hash
+    else
+      epoch_invariant_apply_path_aux epoch right p_next new_parent_parent_hash
+
+val epoch_invariant_apply_path:
+  #bytes:Type0 -> {|crypto_bytes bytes|} -> #tkt:treekem_types bytes ->
+  #l:nat -> #li:leaf_index l 0 ->
+  epoch:nat ->
+  t:treesync bytes tkt l 0 -> p:pathsync bytes tkt l 0 li ->
+  Lemma
+  (requires
+    apply_path_pre #bytes t p /\
+    leaf_node_epoch (get_path_leaf p) <= epoch /\
+    epoch_invariant epoch t
+  )
+  (ensures epoch_invariant epoch (apply_path t p))
+let epoch_invariant_apply_path #bytes #cb #tkt #l #li epoch t p =
+  epoch_invariant_apply_path_aux epoch t p (root_parent_hash #bytes)
+
+val epoch_invariant_augment:
+  #bytes:Type0 -> {|bytes_like bytes|} -> #tkt:treekem_types bytes ->
+  #l:nat -> #i:tree_index l ->
+  epoch_low:nat -> epoch_high:nat ->
+  t:treesync bytes tkt l i ->
+  Lemma
+  (requires epoch_invariant epoch_low t /\ epoch_low <= epoch_high)
+  (ensures epoch_invariant epoch_high t)
+let rec epoch_invariant_augment #bytes #bl #tkt #l #li epoch_low epoch_high t =
+  match t with
+  | TLeaf _ -> ()
+  | TNode _ left right ->
+    epoch_invariant_augment epoch_low epoch_high left;
+    epoch_invariant_augment epoch_low epoch_high right
